@prefix owl: <http://www.w3.org/2002/07/owl#> .
@prefix rdf: <http://www.w3.org/1999/02/22-rdf-syntax-ns#> .
@prefix xml: <http://www.w3.org/XML/1998/namespace> .
@prefix xsd: <http://www.w3.org/2001/XMLSchema#> .
@prefix rdfs: <http://www.w3.org/2000/01/rdf-schema#> .
@prefix skos: <http://www.w3.org/2004/02/skos/core#> .
@prefix vann: <http://purl.org/vocab/vann/> .
@prefix schema:  <http://schema.org/> .
@prefix adr:  <http://kg.artsdata.ca/resource/> .

adr:ArtsdataOrganizationTypes rdf:type owl:NamedIndividual, skos:ConceptScheme ;
  skos:prefLabel "Controlled Vocabulary for organization types" ;
  rdfs:comment "This SKOS Concept Scheme is a controlled vocabulary for organization types used in Artsdata. The goal of this controlled vocabulary is to serve as a base for mapping different types of arts organizations into a common language." ;
  owl:versionInfo "2.0.0";
  vann:preferredNamespacePrefix "adr" ;
  vann:preferredNamespaceUri adr: ;
  schema:dateCreated "2022-04-01"^^xsd:date ;
  schema:dateModified "2022-08-01"^^xsd:date ;
  schema:creator  adr:K1-5 ;
  vann:usageNote <https://culturecreates.github.io/artsdata-data-model/classes/organization.html> ;
  vann:example adr:PerformingGroup ;
  vann:changes <https://github.com/culturecreates/artsdata-data-model/commits/master/ontology/skos-organization-types.ttl> ; 
  skos:hasTopConcept adr:Organization . 

# Copy/paste triples from hidden tab in https://docs.google.com/spreadsheets/d/1z_-7oVZJ1zu61nXa7HzQIHQeYugRGewBSM2VPgfC_NA/edit?usp=sharing
# Pull data from Wikidata to populate adr:WikidataConcept_Q# a schema:DefinedTerm , skos:Concept ; rdfs:label "--name from Wikdiata--" ; schema:url wd:Q### ; schema:termCode "Q##" ; schema:inDefinedTermSet wd:Q#-top-level

adr:Organization  rdf:type owl:NamedIndividual ,  skos:Concept; skos:prefLabel "Organization"@en ; skos:prefLabel "Organisme"@fr ; skos:definition "An organization such as a nonprofit or forprofit corporation, company, school, charity or group."@en ; skos:definition "Une organisme telle qu'une société à but non lucratif ou à but lucratif, une entreprise, une école, un organisme de bienfaisance ou un groupe."@fr ;  skos:closeMatch  adr:WikidataConcept-Q43229  ;  skos:inScheme adr:ArtsdataOrganizationTypes   .
adr:PerformingGroup  rdf:type owl:NamedIndividual ,  skos:Concept   ; skos:broader  adr:Organization; skos:prefLabel "Performing Group"@en ; skos:prefLabel "Groupe de Performance"@fr ; skos:definition "A performing group such as a performing arts company in theatre, music or dance, a band, an orchestra, a performance collective or troupe, a circus."@en ; skos:definition "Un groupe des arts de la scène, tel qu'une compagnie  en théâtre, musique ou danse, un groupe musical, un orchestre, un collectif ou une troupe de spectacle, un cirque."@fr ;  skos:closeMatch  adr:WikidataConcept-Q105815710  ;  skos:inScheme adr:ArtsdataOrganizationTypes   .
adr:TheaterGroup  rdf:type owl:NamedIndividual ,  skos:Concept   ; skos:broader  adr:PerformingGroup; skos:prefLabel "Theatre Group"@en ; skos:prefLabel "Groupe de théâtre"@fr ; skos:definition "A theatre group refers to a group of theatrical performers and creators working together, such as in an acting or theatre company."@en ; skos:definition "Une groupe de théâtre fait référence à un groupe d'artistes et de créateurs de théâtre travaillant ensemble, comme dans une compagnie de théâtre."@fr ;  skos:closeMatch  adr:WikidataConcept-Q2416217  ;  skos:inScheme adr:ArtsdataOrganizationTypes   .
adr:DanceGroup  rdf:type owl:NamedIndividual ,  skos:Concept   ; skos:broader  adr:PerformingGroup; skos:prefLabel "Dance Group"@en ; skos:prefLabel "Groupe de danse"@fr ; skos:definition "A dance group is a group of dancers and associated personnel who work together to perform dances as a performance for a public."@en ; skos:definition "Un groupe de danse est un groupe de danseurs et du personnel associé qui travaillent ensemble pour exécuter des danses en tant que spectacle pour un public."@fr ;  skos:closeMatch  adr:WikidataConcept-Q2393314  ;  skos:inScheme adr:ArtsdataOrganizationTypes   .
adr:BalletCompany  rdf:type owl:NamedIndividual ,  skos:Concept   ; skos:broader  adr:DanceGroup; skos:prefLabel "Ballet Company"@en ; skos:prefLabel "Compagnie de ballet"@fr ; skos:inScheme adr:ArtsdataOrganizationTypes   .
adr:MusicGroup  rdf:type owl:NamedIndividual ,  skos:Concept   ; skos:broader  adr:PerformingGroup; skos:prefLabel "Music Group"@en ; skos:prefLabel "Groupe de musique"@fr ; skos:definition "A musical group, is a group of musicians playing together, such as a band, an orchestra, or a choir. In Schema.org it also includes solo musicians."@en ; skos:definition "Un groupe musical est un groupe de musiciens jouant ensemble, comme dans un groupe, un orchestre ou une chorale. Dans Schema.org, il comprend également un musicien solo."@fr ;  skos:closeMatch  adr:WikidataConcept-Q2088357  ;  skos:inScheme adr:ArtsdataOrganizationTypes   .
adr:Orchestra  rdf:type owl:NamedIndividual ,  skos:Concept   ; skos:broader  adr:MusicGroup; skos:prefLabel "Orchestra"@en ; skos:prefLabel "Orchestre"@fr ; skos:definition "An orchestra is a large instrumental ensemble that combines instruments from different families, including bowed string instruments, woodwinds, brass and percussions typical in classical music. An orchestra may also be refeered to as a syphony orchestra or philharmonic orchestra."@en ; skos:definition "Un orchestre est un grand ensemble instrumental qui combine des instruments de différentes familles, notamment des instruments à cordes frottées, des bois, des cuivres et des percussions typiques de la musique classique. Un orchestre peut également être appelé orchestre symphonique ou orchestre philharmonique."@fr ;  skos:closeMatch  adr:WikidataConcept-Q42998  ;  skos:inScheme adr:ArtsdataOrganizationTypes   .
adr:Circus  rdf:type owl:NamedIndividual ,  skos:Concept   ; skos:broader  adr:PerformingGroup; skos:prefLabel "Circus"@en ; skos:prefLabel "Cirque"@fr ; skos:definition "A circus is a company of performers who put on performances that include a series of acts that showcase a particular skill. A circus may include performances by and is not limited to: clowns, acrobats, trained animals, trapeze artists, stuntmen, musicians, dancers, hoopers, tightrope walkers, jugglers, magicians, ventriloquists, and unicyclists."@en ; skos:definition "Un cirque est une compagnie d'artistes qui organisent des spectacles comprenant une série d'actes mettant en valeur une compétence particulière. Un cirque peut inclure des performances par et n'est pas limité à : clowns, acrobates, animaux entraînés, trapézistes, cascadeurs, musiciens, danseurs, cerceaux, funambules, jongleurs, magiciens, ventriloques et monocyclistes."@fr ;  skos:closeMatch  adr:WikidataConcept-Q47928  ;  skos:inScheme adr:ArtsdataOrganizationTypes   .
adr:OperaCompany  rdf:type owl:NamedIndividual ,  skos:Concept   ; skos:broader  adr:PerformingGroup; skos:prefLabel "Opera Company"@en ; skos:prefLabel "Compagnie d'opéra"@fr ; skos:definition "An arts organization whose primary purpose is to produce and present operas."@en ; skos:definition "Organisme artistique dont le but principal est de produire et de présenter des opéras."@fr ;  skos:closeMatch  adr:WikidataConcept-Q20819922  ;  skos:inScheme adr:ArtsdataOrganizationTypes   .
adr:ArtistRepresentative  rdf:type owl:NamedIndividual ,  skos:Concept   ; skos:broader  adr:Organization; skos:prefLabel "Artist Representative"@en ; skos:prefLabel "Représentant d'artiste"@fr ; skos:definition "An Artist Representative often called Agent, handle the marketing, mangement, sales and negotiations of artists, their works and/or productions."@en ; skos:definition "Un représentant d'artiste souvent appelé agent, s'occupe du marketing, de la gestion, des ventes et des négociations des artistes, de leurs œuvres et/ou productions."@fr ;  skos:closeMatch  adr:WikidataConcept-Q1344174  ;  skos:inScheme adr:ArtsdataOrganizationTypes   .
adr:PresentingOrganization  rdf:type owl:NamedIndividual ,  skos:Concept   ; skos:broader  adr:Organization; skos:prefLabel "Presenter"@en ; skos:prefLabel "Diffuseur"@fr ; skos:definition "An organization or person that finances, organizes and programs the presentation of performing arts and culture events such as: concerts, plays, dance or movies."@en ; skos:definition "UN DIFFUSEUR est une personne (ou une organisme de diffusion) qui offre des représentations artistiques tels que des concerts, des opéras, de la danse, des productions théâtrales en tournée et des spectacles d'humour. Un DIFFUSEUR peut travailler pour une salle spécifique ou organiser une série d'événements qui se déroulent dans une ou plusieurs salles."@fr ;  skos:closeMatch  adr:WikidataConcept-Q7168296  ;  skos:inScheme adr:ArtsdataOrganizationTypes   .
adr:Festival  rdf:type owl:NamedIndividual ,  skos:Concept   ; skos:broader  adr:PresentingOrganization; skos:prefLabel "Festival"@en ; skos:prefLabel "Festival"@fr ; skos:definition "A festival is a type of presenting organization whose primary activity is to put together and promote festivals."@en ; skos:definition "Une série organisée d'événements artistiques et culturels tels que des concerts, des pièces de théâtre, de la danse ou des films."@fr ;  skos:closeMatch  adr:WikidataConcept-Q108669279  ;  skos:inScheme adr:ArtsdataOrganizationTypes   .
adr:ArtsAssociation  rdf:type owl:NamedIndividual ,  skos:Concept   ; skos:broader  adr:Organization; skos:prefLabel "Arts Assocation"@en ; skos:prefLabel "Association d'art"@fr ; skos:definition "An arts assocation is an organization that promotes the interests of its members and/or constituents and provides them with services."@en ; skos:definition "Une association artistique est une organisation d'un groupe de personnes et/ou d'autres organisations qui travaillent ensemble pour travailler sur diverses questions dans le domaine des arts."@fr ;   skos:inScheme adr:ArtsdataOrganizationTypes   .
adr:ArtistUnion  rdf:type owl:NamedIndividual ,  skos:Concept   ; skos:broader  adr:Organization; skos:prefLabel "Artist Union"@en ; skos:prefLabel "Syndicat d'artiste"@fr ; skos:definition "An organized association of professional workers in the arts formed to protect and further their rights and interests."@en ; skos:definition "Un syndicat organisé de travailleurs professionnels du secteur des arts formé pour protéger et promouvoir leurs droits et intérêts."@fr ;   skos:inScheme adr:ArtsdataOrganizationTypes   .
adr:ArtGallery  rdf:type owl:NamedIndividual ,  skos:Concept   ; skos:broader  adr:Organization; skos:prefLabel "Art Gallery"@en ; skos:prefLabel "Galerie d'art"@fr ; skos:definition "An art gallery is an organization that puts together exhibitions of artists works for the purpose of public enjoyment, education and/or sale."@en ; skos:definition "Une galerie d'art est un lieu où les gens peuvent voir et/ou acheter des œuvres d'artistes émergents ou établis."@fr ;   skos:inScheme adr:ArtsdataOrganizationTypes   .
adr:ArtMuseum  rdf:type owl:NamedIndividual ,  skos:Concept   ; skos:broader  adr:Organization; skos:prefLabel "Art Museum"@en ; skos:prefLabel "Musée d'art"@fr ; skos:definition "An art museum is a non-profit institution that acquires, conserves, researches, communicates and exhibits the arts and culture heritage of humanity for the purposes of education, study, and enjoyment."@en ; skos:definition "Un musée d'art est un espace ou un bâtiment dédié utilisé pour exposer des œuvres d'art provenant généralement d'une collection."@fr ;   skos:inScheme adr:ArtsdataOrganizationTypes   .
adr:EducationalOrganization  rdf:type owl:NamedIndividual ,  skos:Concept   ; skos:broader  adr:Organization; skos:prefLabel "Educational Organization"@en ; skos:prefLabel "Organisme Éducatif"@fr ; skos:definition "Educational Organization"@en ; skos:definition "Organisme Éducatif"@fr ;   skos:inScheme adr:ArtsdataOrganizationTypes   .
adr:PerformingArtsSchool  rdf:type owl:NamedIndividual ,  skos:Concept   ; skos:broader  adr:EducationalOrganization; skos:prefLabel "Performing arts school"@en ; skos:prefLabel "École des arts de la scène"@fr ; skos:definition "An educational organization dedicated to teaching subjects concerning the performing arts."@en ; skos:definition "Organisme éducatif voué à l'enseignement de matières concernant les arts de la scène."@fr ;   skos:inScheme adr:ArtsdataOrganizationTypes   .
adr:ArtSchool  rdf:type owl:NamedIndividual ,  skos:Concept   ; skos:broader  adr:EducationalOrganization; skos:prefLabel "Art School"@en ; skos:prefLabel "École d'art"@fr ; skos:definition "An art school is an educational institution with a primary focus on the visual arts."@en ; skos:definition "Une école d'art est un établissement d'enseignement axé principalement sur les arts visuels."@fr ;   skos:inScheme adr:ArtsdataOrganizationTypes   .
adr:GovernmentArtsFunder  rdf:type owl:NamedIndividual ,  skos:Concept   ; skos:broader  adr:Organization; skos:prefLabel "Government Arts Funder"@en ; skos:prefLabel "Bailleur de fonds gouvernemental pour les arts"@fr ; skos:definition "Any government agency and/or government organization dedicated to supporting the arts. They often operate at arms-length from the government to prevent political interference in their decisions."@en ; skos:definition "Toute agence gouvernementale et/ou organisation gouvernementale dédiée au soutien des arts. Ils opèrent souvent sans lien de dépendance avec le gouvernement pour empêcher toute ingérence politique dans leurs décisions."@fr ;   skos:inScheme adr:ArtsdataOrganizationTypes   .
adr:ArtsFoundation  rdf:type owl:NamedIndividual ,  skos:Concept   ; skos:broader  adr:Organization; skos:prefLabel "Arts Foundation"@en ; skos:prefLabel "Fondation des arts"@fr ; skos:definition "An arts foundation is an organization created to support the arts - often with money."@en ; skos:definition "Une fondation des arts est une organisation créée pour soutenir les arts - souvent avec de l'argent."@fr ;   skos:inScheme adr:ArtsdataOrganizationTypes   .