@prefix owl: <http://www.w3.org/2002/07/owl#> .
@prefix rdf: <http://www.w3.org/1999/02/22-rdf-syntax-ns#> .
@prefix xml: <http://www.w3.org/XML/1998/namespace> .
@prefix xsd: <http://www.w3.org/2001/XMLSchema#> .
@prefix rdfs: <http://www.w3.org/2000/01/rdf-schema#> .
@prefix skos: <http://www.w3.org/2004/02/skos/core#> .
@prefix vann: <http://purl.org/vocab/vann/> .
@prefix schema:  <http://schema.org/> .
@prefix adr:  <http://kg.artsdata.ca/resource/> .

adr:ArtsdataOrganizationTypes rdf:type owl:NamedIndividual, skos:ConceptScheme ;
  skos:prefLabel "Controlled Vocabulary for organization types" ;
  rdfs:comment "This SKOS Concept Scheme is a controlled vocabulary for organization types used in Artsdata. The goal of this controlled vocabulary is to serve as a base for mapping different types of arts organizations into a common language." ;
  owl:versionInfo "3.0.0";
  vann:preferredNamespacePrefix "adr" ;
  vann:preferredNamespaceUri adr: ;
  schema:dateCreated "2022-04-01"^^xsd:date ;
  schema:dateModified "2023-03-14"^^xsd:date ;
  schema:creator  adr:K16-211 ;
  vann:usageNote <https://culturecreates.github.io/artsdata-data-model/classes/organization.html> ;
  vann:example adr:PerformingArtsCompany ;
  vann:changes <https://github.com/culturecreates/artsdata-data-model/commits/master/ontology/skos-organization-types.ttl> ; 
  skos:hasTopConcept adr:Organization . 

# Copy/paste triples from 'Generate triples' tab in https://docs.google.com/spreadsheets/d/1wPzZI3G48q02H_II91Bs6ljZFbC0KcSAPzDDK0dtGN8/edit#gid=1933025380
# TODO: Work needed to add skos mapping to other vocabularies

adr:Organization  rdf:type owl:NamedIndividual ,  skos:Concept   ; skos:broader  adr:Agent; skos:prefLabel "Organization"@en ; skos:prefLabel "Organisme"@fr ; skos:definition "A structured group of people, united by a common purpose. This includes both groups that are formally structured as a legal body (e.g., a not-for-profit corporation) as well as those that are informally structured, but otherwise act together."@en ; skos:definition "Un groupe structuré de personnes, unies par un objectif commun. Il s'agit aussi bien de groupes structurés officiellement comme une entité juridique (par exemple, une entreprise à but non lucratif) et de groupes structurés de manière informelle, mais qui par ailleurs agissent ensemble."@fr ;   skos:inScheme adr:ArtsdataOrganizationTypes   .
adr:ArtsOrganization  rdf:type owl:NamedIndividual ,  skos:Concept   ; skos:broader  adr:Organization; skos:prefLabel "Arts Organization"@en ; skos:prefLabel "Organisme artistique"@fr ; skos:definition "An organization whose primary activity is to create, perform, present and/or promote the visual, performing and/or literary arts. It does not refer to an organization whose purpose is instructional and educational."@en ; skos:definition "Une organisation dont l’activité principal est de créer, exécuter, présenter et/ou promouvoir les arts visuels, de la scène et/ou littéraires. Il ne fait pas référence à une organisation dont le but est pédagogique et éducatif."@fr ;   skos:inScheme adr:ArtsdataOrganizationTypes   .
adr:PerformingArtsCompany  rdf:type owl:NamedIndividual ,  skos:Concept   ; skos:broader  adr:ArtsOrganization; skos:prefLabel "Performing Arts Company"@en ; skos:prefLabel "Compagnie en arts de la scène"@fr ; skos:definition "A group of artists and related personnel whose primary activity is creating/producing theatrical productions, dance productions, concerts, circuses, variety shows and/or other performing arts events."@en ; skos:definition "Un groupe d'artistes et personnel associé dont l’activité principal est de créer/produire les productions théâtrales, productions de la danse, les concerts, les cirques, les spectacles de variétés et/ou d’autres événements des arts de la scène."@fr ;   skos:inScheme adr:ArtsdataOrganizationTypes   .
adr:TheatreCompany  rdf:type owl:NamedIndividual ,  skos:Concept   ; skos:broader  adr:PerformingArtsCompany; skos:prefLabel "Theatre Company"@en ; skos:prefLabel "Compagnie de théâtre"@fr ; skos:definition "A group of artists and associated personnel who mainly create and/or perform plays, puppet shows, and/or similar theatrical productions. It does not refer to groups who primarily produce musicals, ballets or operas."@en ; skos:definition "Un groupe d’artistes et personnel associé qui créent et/ou interprétent principalement les pièces, les spectacles de marionettes, et/ou les productions théâtrales similaires. Il ne fait pas référence aux groupes qui produisent principalement les comédies musicales, les ballets ou les opéras."@fr ;   skos:inScheme adr:ArtsdataOrganizationTypes   .
adr:MusicalTheatreCompany  rdf:type owl:NamedIndividual ,  skos:Concept   ; skos:broader  adr:PerformingArtsCompany; skos:prefLabel "Musical Theatre Company"@en ; skos:prefLabel "Compagnie de comédies musicales"@fr ; skos:definition "A group of artists and associated personnel who mainly create and/or perform musicals and/or similar theatrical productions. These productions are characterized by a combination of music, dance, and spoken and sung dialogue."@en ; skos:definition "Un groupe d'artistes et personnel associé qui créent et/ou interprétent principalement des comédies musicales et/ou autres productions similaires. Ces productions sont caractérisées par la musique, la danse et les dialogues parlés et chantés."@fr ;   skos:inScheme adr:ArtsdataOrganizationTypes   .
adr:OperaCompany  rdf:type owl:NamedIndividual ,  skos:Concept   ; skos:broader  adr:PerformingArtsCompany; skos:prefLabel "Opera Company"@en ; skos:prefLabel "Compagnie d'opéra"@fr ; skos:definition "A group of artists and associated personnel who mainly create and/or perform operas. These musical/theatrical productions contain dialogue that is almost always sung."@en ; skos:definition "Un groupe d'artistes et personnel associé qui créent et/ou interprétent principalement des opéras. Ces productions musicales/théâtrales contient les dialogues qui sont presque toujours chantés."@fr ;   skos:inScheme adr:ArtsdataOrganizationTypes   .
adr:DanceCompany  rdf:type owl:NamedIndividual ,  skos:Concept   ; skos:broader  adr:PerformingArtsCompany; skos:prefLabel "Dance Company"@en ; skos:prefLabel "Compagnie de danse"@fr ; skos:definition "A group of artists and associated personnel who mainly create and/or perform dance productions. These types of stage productions are characterized by rhythmic movement, usually set to music."@en ; skos:definition "Un groupe d’artistes et personnel associé qui créent et/ou intérpretent principalement les spectacles de la danse. Ces types de productions scéniques sont caractérisés par le mouvement rythmique, généralement mis en musique."@fr ;   skos:inScheme adr:ArtsdataOrganizationTypes   .
adr:MusicGroup  rdf:type owl:NamedIndividual ,  skos:Concept   ; skos:broader  adr:PerformingArtsCompany; skos:prefLabel "Music Group"@en ; skos:prefLabel "Groupe de musique"@fr ; skos:definition "A group of vocalists, instrumentalists and/or similar artists who mainly perform together. In Schema.org it also includes solo musicians."@en ; skos:definition "Un groupe de vocalistes, instrumentistes et/ou artistes similares qui jouent principalement ensemble. Dans Schema.org, il comprend également des artistes solo."@fr ;   skos:inScheme adr:ArtsdataOrganizationTypes   .
adr:CircusCompany  rdf:type owl:NamedIndividual ,  skos:Concept   ; skos:broader  adr:PerformingArtsCompany; skos:prefLabel "Circus Company"@en ; skos:prefLabel "Compagnie de cirque"@fr ; skos:definition "A group of specialized artists and associated personnel who mainly showcase acts of human skill and/or daring. These may include (but aren’t limited to) acrobatics, stunts, clownery, animal training, and magic."@en ; skos:definition "Un groupe d'artistes spécialisés et personnel associé qui présentent principalement des actes de compétence et/ou d’audace humaine. Ceux-ci peuvent comprendre (mais pas uniquement) d'acrobaties, de cascades, de clownerie, de dressage d'animaux et de magie."@fr ;   skos:inScheme adr:ArtsdataOrganizationTypes   .
adr:ArtistRepresentative  rdf:type owl:NamedIndividual ,  skos:Concept   ; skos:broader  adr:ArtsOrganization; skos:prefLabel "Artist Representative"@en ; skos:prefLabel "Représentant d'artiste"@fr ; skos:definition "A person or organization whose primary activity is to represent artists in contract negotiations, manage or organize their financial affairs, and/or generally promote their works."@en ; skos:definition "Une personne ou une organisation dont l’activité principale est de represénter les artistes dans la négociation des contrats, gèrer ou organiser leurs finances, et s’occuper habituellement de promouvoir leur travail."@fr ;   skos:inScheme adr:ArtsdataOrganizationTypes   .
adr:PresentingOrganization  rdf:type owl:NamedIndividual ,  skos:Concept   ; skos:broader  adr:ArtsOrganization; skos:prefLabel "Presenter"@en ; skos:prefLabel "Diffuseur"@fr ; skos:definition "An organization or person whose primary activity is to organize, program and/or promote productions that are created/performed by others."@en ; skos:definition "Une organisation (ou une personne) dont l’activité primaire est d’organiser, programmer et/ou promouvoir des productions qui sont crées/interpretées par des autres."@fr ;   skos:inScheme adr:ArtsdataOrganizationTypes   .
adr:FestivalOrganization  rdf:type owl:NamedIndividual ,  skos:Concept   ; skos:broader  adr:PresentingOrganization; skos:prefLabel "Festival Organization"@en ; skos:prefLabel "Organisme de festival"@fr ; skos:definition "A presenting organization whose primary activity is to program and promote a collection of cultural events based around a common theme. This may include (but isn’t limited to) concerts, plays, dance productions, etc."@en ; skos:definition "Une organisation de diffusion dont l’activité primaire est de programmer et promouvoir une collection d’événements culturels qui sont axés sur un theme commun. Elle peut inclure (mais pas uniquement) des concerts, des pièces de théâtre, des productions de la danse, etc."@fr ;   skos:inScheme adr:ArtsdataOrganizationTypes   .
adr:ArtsServiceOrganization  rdf:type owl:NamedIndividual ,  skos:Concept   ; skos:broader  adr:ArtsOrganization; skos:prefLabel "Arts Service Organization"@en ; skos:prefLabel "Organisme de services aux arts"@fr ; skos:definition "An organization whose primary activity is to provide services to individuals and/or organizational members within an industry/sector, including promoting their interests."@en ; skos:definition "Une organisation dont l’activité principale est de fournir des services aux membres individuels et/ou organisationnels dans une industrie/un secteur, y compris la promotion de leurs intérêts."@fr ;   skos:inScheme adr:ArtsdataOrganizationTypes   .
adr:ArtistUnion  rdf:type owl:NamedIndividual ,  skos:Concept   ; skos:broader  adr:ArtsOrganization; skos:prefLabel "Artist Union"@en ; skos:prefLabel "Syndicat d'artiste"@fr ; skos:definition "An organization whose primary activity is to regulate labour relations between employees and employers and promote employee interests."@en ; skos:definition "Une organisation dont l’activité principale est de régler les relations de travail entre employés et employeurs et de promouvoir les intérêts des employés."@fr ;   skos:inScheme adr:ArtsdataOrganizationTypes   .
adr:ArtMuseum  rdf:type owl:NamedIndividual ,  skos:Concept   ; skos:broader  adr:ArtsOrganization; skos:prefLabel "Art Museum"@en ; skos:prefLabel "Musée d'art"@fr ; skos:definition "An organization whose primary activity is to acquire, conserve, research, exhibit and promote the arts and cultural heritage of humanity."@en ; skos:definition "Une organisation dont l’activité principale est d’acquérir, conserver, rechercher, communiquer et exposer les arts et le patrimoine culturel de l’humanité."@fr ;   skos:inScheme adr:ArtsdataOrganizationTypes   .
adr:CommunityOrganization  rdf:type owl:NamedIndividual ,  skos:Concept   ; skos:broader  adr:Organization; skos:prefLabel "Community Organization"@en ; skos:prefLabel "Organisme communautaire"@fr ; skos:definition "An organization whose primary activity is to promote the social and/or cultural wellbeing of its community members."@en ; skos:definition "Une organisation dont l’activité principale est de promouvoir le bien-être social et/ou culturel des membres de la collectivité."@fr ;   skos:inScheme adr:ArtsdataOrganizationTypes   .
adr:EducationalOrganization  rdf:type owl:NamedIndividual ,  skos:Concept   ; skos:broader  adr:Organization; skos:prefLabel "Educational Organization"@en ; skos:prefLabel "Organisme éducatif"@fr ; skos:definition "An organization whose primary activity is to provide instruction and training in one particular subject or a variety of subjects."@en ; skos:definition "Une organisation dont l’activité principale est de fournir l’instruction et la formation dans un sujet particulier ou une variété de sujets."@fr ;   skos:inScheme adr:ArtsdataOrganizationTypes   .
adr:PerformingArtsSchool  rdf:type owl:NamedIndividual ,  skos:Concept   ; skos:broader  adr:EducationalOrganization; skos:prefLabel "Performing Arts School"@en ; skos:prefLabel "École des arts de la scène"@fr ; skos:definition "An educational institution whose primary activity is to provide instruction in technical and/or professional skills in the performing arts."@en ; skos:definition "Un établissement d’enseignement dont l’activité principale est de fournir la formation dans les competences techniques et/ou professionnels dans le domaine des arts de la scène."@fr ;   skos:inScheme adr:ArtsdataOrganizationTypes   .
adr:ArtSchool  rdf:type owl:NamedIndividual ,  skos:Concept   ; skos:broader  adr:EducationalOrganization; skos:prefLabel "Art School"@en ; skos:prefLabel "École d'art"@fr ; skos:definition "An educational institution whose primary activity is to provide instruction in the visual arts."@en ; skos:definition "Un établissement d'enseignement dont l’activité principale est de fournir la formation dans les arts visuels."@fr ;   skos:inScheme adr:ArtsdataOrganizationTypes   .
adr:PublicFunder  rdf:type owl:NamedIndividual ,  skos:Concept   ; skos:broader  adr:Organization; skos:prefLabel "Public Funder"@en ; skos:prefLabel "Bailleur de fonds publics"@fr ; skos:definition "A government agency and/or organization whose primary activity is to financially support a program, organization or domain. They often operate at arms-length from the government to prevent political interference in their decisions."@en ; skos:definition "Un agence et/ou une organisation gouvernemental dont l’activité principale est de fournir le soutien à un programme, un organisme ou un domaine. Ils opèrent souvent sans lien de dépendance avec le gouvernement pour empêcher toute ingérence politique dans leurs décisions."@fr ;   skos:inScheme adr:ArtsdataOrganizationTypes   .
adr:PublicArtsFunder  rdf:type owl:NamedIndividual ,  skos:Concept   ; skos:broader  adr:PublicFunder; skos:prefLabel "Public Arts Funder"@en ; skos:prefLabel "Bailleur de fonds publics pour les arts"@fr ; skos:definition "A public funder who mainly supports arts programs, arts organizations or the arts sector as a whole."@en ; skos:definition "Un bailleur de fonds publics qui soutiennent principalement les programmes d'arts, les organismes artistiques et/ou le domaine des arts dans son ensemble."@fr ;   skos:inScheme adr:ArtsdataOrganizationTypes   .
adr:Foundation  rdf:type owl:NamedIndividual ,  skos:Concept   ; skos:broader  adr:Organization; skos:prefLabel "Foundation"@en ; skos:prefLabel "Fondation"@fr ; skos:definition "An organization whose primary activity is to provide long-term financial support for charitable causes."@en ; skos:definition "Une organisation dont l'activité principale est de fournir un soutien financier aux causes charitables."@fr ;   skos:inScheme adr:ArtsdataOrganizationTypes   .
adr:ArtsFoundation  rdf:type owl:NamedIndividual ,  skos:Concept   ; skos:broader  adr:Foundation; skos:prefLabel "Arts Foundation"@en ; skos:prefLabel "Fondation des arts"@fr ; skos:definition "A foundation who mainly provides financial support for a specific arts organization, for multiple organizations or for the arts sector as a whole. "@en ; skos:definition "Une fondation qui fournissent principalement le soutien financier à un organisme artistique specifique, aux multiples organismes ou au domaine des arts dans son ensemble. "@fr ;   skos:inScheme adr:ArtsdataOrganizationTypes   .
