@prefix owl: <http://www.w3.org/2002/07/owl#> .
@prefix rdf: <http://www.w3.org/1999/02/22-rdf-syntax-ns#> .
@prefix xml: <http://www.w3.org/XML/1998/namespace> .
@prefix xsd: <http://www.w3.org/2001/XMLSchema#> .
@prefix rdfs: <http://www.w3.org/2000/01/rdf-schema#> .
@prefix skos: <http://www.w3.org/2004/02/skos/core#> .
@prefix vann: <http://purl.org/vocab/vann/> .
@prefix schema:  <http://schema.org/> .
@prefix adr:  <http://kg.artsdata.ca/resource/> .
@prefix ado:  <http://kg.artsdata.ca/ontology/> .
@prefix spt: <http://scenepro.ca/taxonomies/disciplines-asq#> . 
@prefix footlight: <http://lod.footlight.io/resource/> .

adr:ArtsdataEventTypes rdf:type owl:NamedIndividual, skos:ConceptScheme ;
  skos:prefLabel "Controlled Vocabulary for event types" ;
  rdfs:comment "This SKOS Concept Scheme is a controlled vocabulary for event types (types, categories, disciplines) in Artsdata. The goal of this controlled vocabulary is to serve as a base for mapping different arts organization's event types so events can be reused in event calendars." ;
  owl:versionInfo "3.4.5";
  vann:preferredNamespacePrefix "adr" ;
  vann:preferredNamespaceUri adr: ;
  schema:dateCreated "2021-08-10"^^xsd:date ;
  schema:dateModified "2025-02-06"^^xsd:date ;
  schema:creator  adr:K1-5 ;
  vann:usageNote <https://culturecreates.github.io/artsdata-data-model/classes/event.html> ;
  vann:example adr:PerformingArtsEvent ;
  vann:changes <https://github.com/culturecreates/artsdata-data-model/commits/master/ontology/skos-event-types.ttl> ; 
  skos:hasTopConcept adr:Event . 

ado:EventType rdf:type rdfs:Class ; rdfs:label "Artsdata Event types" ; rdfs:comment "Artsdata Event types defined as a class in addition to using SKOS. This Artsdata specific class facilitates reconciliation, instead of reconiling skos:Concepts is it more direct to reconcile individuals that are ado:EventType." .
## Copy below from spreadsheet https://docs.google.com/spreadsheets/d/1ud_kVTE8C97ZMoe1uYGQ6rW_dodKqsbqiCutLLHO9jo/edit#gid=0
adr:ChildrensEvent  rdf:type owl:NamedIndividual , skos:Concept , ado:EventType ; skos:broader  adr:Event ; skos:prefLabel "Children's Event"@en ; skos:prefLabel "Événement pour enfants"@fr ; skos:altLabel "Family"@en ; skos:altLabel "Famille"@fr ; skos:definition "Event type for children."@en ; skos:definition "Type d'événement : Événement pour enfants."@fr ;  skos:closeMatch schema:ChildrensEvent   ; skos:inScheme adr:ArtsdataEventTypes   .
adr:Event  rdf:type owl:NamedIndividual , skos:Concept , ado:EventType ; skos:prefLabel "Event"@en ; skos:prefLabel "Événement"@fr ; skos:definition "An event is a happening that occurs at a certain time and location. Examples include and are not limited to a: performance, concert, conference, festival, exhibition and/or social gathering."@en ; skos:definition "Un événement est un événement qui se produit à un certain moment et à un certain endroit. Les exemples incluent, sans s'y limiter : une performance, un concert, une conférence, un festival, une exposition et/ou un événement social."@fr ; skos:note "https://github.com/culturecreates/artsdata-data-model/issues/16" ;  skos:closeMatch schema:Event   ; skos:inScheme adr:ArtsdataEventTypes   .
adr:EventSeries  rdf:type owl:NamedIndividual , skos:Concept , ado:EventType ; skos:broader  adr:Event ; skos:prefLabel "Event Series"@en ; skos:prefLabel "Série d'événements"@fr ; skos:definition "An event series is a series of events such as mutiple performances of a same show, or different events grouped by theme. In Schema, included events relate with the series using a superEvent property."@en ; skos:definition "Une série d'événements est une série d'événements connexes tels que plusieurs représentations d'un même spectacle, ou des événements sur un thème. Dans Schema, les événements inclus sont liés à la série à l'aide d'une propriété superEvent."@fr ;  skos:closeMatch schema:EventSeries   ; skos:inScheme adr:ArtsdataEventTypes   .
adr:ExhibitionEvent  rdf:type owl:NamedIndividual , skos:Concept , ado:EventType ; skos:broader  adr:Event ; skos:prefLabel "Exhibition"@en ; skos:prefLabel "Exposition"@fr ; skos:definition "An exhibition is a type of event where a collection of objects put together are curated under a theme for the purpose of being presented to a public."@en ; skos:definition "Une exposition est un type d'événement où une collection d'objets rassemblés est organisée sous un thème dans le but d'être présentée à un public."@fr ;  skos:closeMatch schema:ExhibitionEvent   ;  skos:closeMatch footlight:6418bbc65e4d4e0066a2e5ee ;   skos:closeMatch footlight:63c01b741c6b6c005aad86c2 ;   skos:closeMatch footlight:65b2575b8468f40064831051 ;   skos:closeMatch <https://www.laval.ca/d1a01a8d-f1ab-4bf6-aa31-c2b0df375121> ;  skos:inScheme adr:ArtsdataEventTypes   .
adr:Festival  rdf:type owl:NamedIndividual , skos:Concept , ado:EventType ; skos:broader  adr:Event ; skos:prefLabel "Festival"@en ; skos:prefLabel "Festival"@fr ; skos:definition "A festival is an organized set of events."@en ; skos:definition "Un festival est un ensemble organisé d'événements."@fr ;  skos:closeMatch schema:Festival   ;  skos:closeMatch footlight:6418ca425e4d4e0066a2ee9f ;  skos:inScheme adr:ArtsdataEventTypes   .
adr:MasterclassEvent  rdf:type owl:NamedIndividual , skos:Concept , ado:EventType ; skos:broader  adr:Event ; skos:prefLabel "Masterclass"@en ; skos:prefLabel "Cours de maître"@fr ; skos:definition "A masterclass is a class given by an expert in a specific discipline: such as in music, dance, singing, painting or playwrighting."@en ; skos:definition "Une masterclass est un cours donné par un expert dans une discipline spécifique : comme la musique, la danse, le chant, la peinture ou la dramaturgie."@fr ; skos:inScheme adr:ArtsdataEventTypes   .
adr:PerformingArtsEvent  rdf:type owl:NamedIndividual , skos:Concept , ado:EventType ; skos:broader  adr:Event ; skos:prefLabel "Performing Arts Event"@en ; skos:prefLabel "Événement des arts de la scène"@fr ; skos:definition "A performing arts event is performing arts work performed for an audience.  It includes a range of performing arts disciplines and genres such as: theatre, ballet, opera, musical theatre, concerts, circus and dance."@en ; skos:definition "Un événement des arts de la scène est une œuvre des arts de la scène exécutée pour un public. Il comprend une gamme de disciplines et de genres des arts de la scène tels que : le théâtre, le ballet, l'opéra, le théâtre musical, les concerts, le cirque et la danse."@fr ; skos:inScheme adr:ArtsdataEventTypes   .
adr:PublicationEvent  rdf:type owl:NamedIndividual , skos:Concept , ado:EventType ; skos:broader  adr:Event ; skos:prefLabel "Publication Event"@en ; skos:prefLabel "Événement de publication"@fr ; skos:definition "Aligning with Schema.org, a PublicationEvent is related to the event of publication of any CreativeWork of any type such as: a broadcast event, an on-demand event, a book/journal publication via a variety of delivery media."@en ; skos:definition "Conformément à Schema.org, un événement de publication est lié à l'événement de publication de tout travail créatif de tout type, tel que : un événement de diffusion, un événement à la demande, une publication de livre/journal via une variété de méthodes médiatiques."@fr ;  skos:closeMatch schema:PublicationEvent   ; skos:inScheme adr:ArtsdataEventTypes   .
adr:RehearsalEvent  rdf:type owl:NamedIndividual , skos:Concept , ado:EventType ; skos:broader  adr:Event ; skos:prefLabel "Rehearsal"@en ; skos:prefLabel "Répétition"@fr ; skos:definition "A rehearsal event is an event where the preparation of a performance  is presented to a public."@en ; skos:definition "Un événement de répétition est un événement où la préparation d'un spectacle est présentée à un public."@fr ; skos:inScheme adr:ArtsdataEventTypes   .
adr:ResidencyActivity  rdf:type owl:NamedIndividual , skos:Concept , ado:EventType ; skos:broader  adr:Event ; skos:prefLabel "Residency"@en ; skos:prefLabel "Résidence"@fr ; skos:definition "A residency activity is an activity where a sponsor, usually a performing arts organization with access  theatre or venue facility, supports the work of artists by providing resources."@en ; skos:definition "Une activité de résidence est une activité où un sponsor, généralement un organisme des arts de la scène avec accès à un théâtre ou à une salle, soutient le travail des artistes en fournissant des ressources."@fr ; skos:inScheme adr:ArtsdataEventTypes   .
adr:ScreeningEvent  rdf:type owl:NamedIndividual , skos:Concept , ado:EventType ; skos:broader  adr:Event ; skos:prefLabel "Screening"@en ; skos:prefLabel "Projection"@fr ; skos:altLabel "Film, Cinema"@en ; skos:altLabel "Film, Cinéma"@fr ; skos:definition "The presentation or showing of a film or video."@en ; skos:definition "La présentation ou la projection d'un film ou d'une vidéo."@fr ;  skos:closeMatch schema:ScreeningEvent   ; skos:inScheme adr:ArtsdataEventTypes   .
adr:SocialEvent  rdf:type owl:NamedIndividual , skos:Concept , ado:EventType ; skos:broader  adr:Event ; skos:prefLabel "Social Event"@en ; skos:prefLabel "Événement social"@fr ; skos:definition "A social event is an event organized and planned for a larger group of people."@en ; skos:definition "Un événement social est un événement organisé et planifié pour un plus grand groupe de personnes."@fr ;  skos:closeMatch schema:SocialEvent   ; skos:inScheme adr:ArtsdataEventTypes   .
adr:VisualArtsEvent  rdf:type owl:NamedIndividual , skos:Concept , ado:EventType ; skos:broader  adr:Event ; skos:prefLabel "Visual and media arts event"@en ; skos:prefLabel "Evénement des arts visuels et médiatiques"@fr ; skos:definition "Is any event that is related to the discpline of visual arts that includes and is not limited to: ceramics, drawing, painting, photography, digital arts, scuplture, textile arts, conceptual art, film-making, architecture and performance arts."@en ; skos:definition "Est tout événement lié à la discipline des arts visuels qui comprend et ne se limite pas à : la céramique, le dessin, la peinture, la photographie, les arts numériques, la sculpture, les arts textiles, l'art conceptuel, la réalisation de films, l'architecture et les arts de la scène."@fr ;  skos:closeMatch schema:VisualArtsEvent   ; skos:inScheme adr:ArtsdataEventTypes   .
adr:WorkshopEvent  rdf:type owl:NamedIndividual , skos:Concept , ado:EventType ; skos:broader  adr:Event ; skos:prefLabel "Workshop"@en ; skos:prefLabel "Atelier"@fr ; skos:definition "A meeting of people to discuss or practice a specific subject or activity."@en ; skos:definition "Une réunion de personnes afin de discuter ou pratiquer un sujet ou une activité spécifique."@fr ; skos:inScheme adr:ArtsdataEventTypes   .
adr:CircusPerformance  rdf:type owl:NamedIndividual , skos:Concept , ado:EventType ; skos:broader  adr:PerformingArtsEvent ; skos:prefLabel "Circus"@en ; skos:prefLabel "Cirque"@fr ; skos:definition "A circus is a form of entertainment and spectacle that involves a series of short acts to display human skill, daring, humour and sometimes skilled tricks involving animals.  Often performed in the round under a large tent."@en ; skos:definition "Un cirque est une forme de divertissement et de spectacle qui implique une série de courts numéros pour montrer l'habileté humaine, l'audace, l'humour et parfois des tours impliquant des animaux. Souvent exécuté en rond sous une grande tente."@fr ; skos:note "https://github.com/culturecreates/artsdata-data-model/issues/7" ;  skos:exactMatch spt:Cirque ;  skos:inScheme adr:ArtsdataEventTypes   .
adr:ComedyPerformance  rdf:type owl:NamedIndividual , skos:Concept , ado:EventType ; skos:broader  adr:PerformingArtsEvent ; skos:prefLabel "Comedy"@en ; skos:prefLabel "Humour"@fr ; skos:definition "A comedy performance is a form of live entertainment intended to make an audience laugh."@en ; skos:definition "Une comédie est une forme de divertissement destinée à faire rire le public."@fr ;  skos:closeMatch schema:ComedyEvent   ;  skos:exactMatch spt:Humour ;  skos:inScheme adr:ArtsdataEventTypes   .
adr:DancePerformance  rdf:type owl:NamedIndividual , skos:Concept , ado:EventType ; skos:broader  adr:PerformingArtsEvent ; skos:prefLabel "Dance"@en ; skos:prefLabel "Danse"@fr ; skos:definition "A dance performance is dance performed for an audience."@en ; skos:definition "Un spectacle de danse est une danse exécutée pour un public."@fr ; skos:note "https://github.com/culturecreates/artsdata-data-model/issues/23" ;  skos:closeMatch schema:DanceEvent   ;  skos:exactMatch spt:Danse ;  skos:inScheme adr:ArtsdataEventTypes   .
adr:MusicalTheatrePerformance  rdf:type owl:NamedIndividual , skos:Concept , ado:EventType ; skos:broader  adr:PerformingArtsEvent ; skos:prefLabel "Musical Theatre"@en ; skos:prefLabel "Théâtre musical"@fr ; skos:altLabel "Broadway"@en ; skos:altLabel "Broadway"@fr ; skos:definition "Musical theatre is a form of theatrical performance that combines music, singing, dialogue, acting and dance to tell a story."@en ; skos:definition "Le théâtre musical est une forme de représentation théâtrale qui combine musique, chant, dialogue, jeu d'acteur et danse pour raconter une histoire."@fr ;  skos:closeMatch schema:TheaterEvent   ;  skos:closeMatch spt:Musical ;   skos:broadMatch spt:Theatre ;  skos:inScheme adr:ArtsdataEventTypes   .
adr:MusicPerformance  rdf:type owl:NamedIndividual , skos:Concept , ado:EventType ; skos:broader  adr:PerformingArtsEvent ; skos:prefLabel "Music"@en ; skos:prefLabel "Musique"@fr ; skos:definition "A music performance or concert is music performed for an audience."@en ; skos:definition "Une performance musique ou un concert est musique jouée pour un public."@fr ;  skos:closeMatch schema:MusicEvent   ;  skos:exactMatch spt:Musique ;  skos:inScheme adr:ArtsdataEventTypes   .
adr:OperaPerformance  rdf:type owl:NamedIndividual , skos:Concept , ado:EventType ; skos:broader  adr:PerformingArtsEvent ; skos:prefLabel "Opera"@en ; skos:prefLabel "Opéra"@fr ; skos:definition "Opera is a form of theatrical performance where music is the fundamental component. Dramatic roles are taken by singers who sing throughout the performance to convey the story."@en ; skos:definition "L'opéra est une forme de représentation théâtrale où la musique est la composante fondamentale. Les rôles dramatiques sont joués par des chanteurs qui chantent tout au long de la représentation pour transmettre l'histoire."@fr ;  skos:closeMatch schema:MusicEvent   ;  skos:exactMatch spt:Opera ;  skos:inScheme adr:ArtsdataEventTypes   .
adr:SpokenWordPerformance  rdf:type owl:NamedIndividual , skos:Concept , ado:EventType ; skos:broader  adr:PerformingArtsEvent ; skos:prefLabel "Spoken Word"@en ; skos:prefLabel "Arts de la parole"@fr ; skos:altLabel "Création parlée"@fr ; skos:definition "A spoken word is a designation for poetry that is performed for a public."@en ; skos:definition "Prestation artistique axée sur l'oralisation d'un texte, qu'il soit poétique ou autre."@fr ; skos:note "https://github.com/culturecreates/artsdata-data-model/issues/101" ;  skos:closeMatch schema:TheaterEvent   ;  skos:exactMatch spt:ArtDeLaParole ;  skos:inScheme adr:ArtsdataEventTypes   .
adr:TheatrePerformance  rdf:type owl:NamedIndividual , skos:Concept , ado:EventType ; skos:broader  adr:PerformingArtsEvent ; skos:prefLabel "Theatre"@en ; skos:prefLabel "Théâtre"@fr ; skos:definition "A theatre performance is theatre work performed for an audience."@en ; skos:definition "Une représentation théâtrale est une pièce de théâtre jouée pour un public."@fr ;  skos:closeMatch schema:TheaterEvent   ;  skos:exactMatch spt:Theatre ;  skos:inScheme adr:ArtsdataEventTypes   .
adr:BroadcastEvent  rdf:type owl:NamedIndividual , skos:Concept , ado:EventType ; skos:broader  adr:PublicationEvent ; skos:prefLabel "Broadcast"@en ; skos:prefLabel "Diffusion"@fr ; skos:definition "It is a one-to-many distribution of video and/or audio content via a electronic mass communication method. The content may be livestreamed or pre-recorded."@en ; skos:definition "Il s'agit d'une distribution un-à-plusieurs de contenu vidéo et/ou audio via une méthode de communication électronique de masse. Le contenu peut être diffusé en direct ou pré-enregistré."@fr ; skos:note "https://github.com/culturecreates/artsdata-data-model/issues/30" ;  skos:closeMatch schema:BroadcastEvent   ; skos:inScheme adr:ArtsdataEventTypes   .
adr:LiveBroadcastEvent  rdf:type owl:NamedIndividual , skos:Concept , ado:EventType ; skos:broader  adr:BroadcastEvent ; skos:prefLabel "Live Stream"@en ; skos:prefLabel "Diffusion en direct"@fr ; skos:definition "A livestream broadcast of video and/or audio content via a electronic mass communication method."@en ; skos:definition "Une diffusion en direct de contenu vidéo et/ou audio via un procédé de communication électronique de masse."@fr ; skos:inScheme adr:ArtsdataEventTypes   .
adr:OnDemand  rdf:type owl:NamedIndividual , skos:Concept , ado:EventType ; skos:broader  adr:PublicationEvent ; skos:prefLabel "On Demand"@en ; skos:prefLabel "Sur demande"@fr ; skos:definition "As per Schema.org, this is a publication event during which a program (e.g. catch-up TV or radio podcast) is available on-demand."@en ; skos:definition "Selon Schema.org, il s'agit d'un événement de publication au cours duquel un programme (par exemple, une télévision de rattrapage ou un podcast radio) est disponible à la demande."@fr ;  skos:closeMatch schema:OnDemandEvent   ; skos:inScheme adr:ArtsdataEventTypes   .
adr:PostshowTalk  rdf:type owl:NamedIndividual , skos:Concept , ado:EventType ; skos:broader  adr:Event ; skos:prefLabel "Postshow Talk"@en ; skos:prefLabel "Conférence après-spectacle"@fr ; skos:definition "An informative talk with an audience after a performance"@en ; skos:definition "Une discussion informative avec un public après une représentation"@fr ;  skos:closeMatch schema:Event   ; skos:inScheme adr:ArtsdataEventTypes   .
adr:PreshowTalk  rdf:type owl:NamedIndividual , skos:Concept , ado:EventType ; skos:broader  adr:Event ; skos:prefLabel "Preshow Talk"@en ; skos:prefLabel "Conférence avant-spectacle"@fr ; skos:definition "An informative talk with an audience before a performance"@en ; skos:definition "Une discussion informative avec un public avant une représentation"@fr ;  skos:closeMatch schema:Event   ; skos:inScheme adr:ArtsdataEventTypes   .
adr:PerformanceArt  rdf:type owl:NamedIndividual , skos:Concept , ado:EventType ; skos:broader  adr:VisualArtsEvent ; skos:prefLabel "Performance Art"@en ; skos:prefLabel "Art performance"@fr ; skos:definition "An art form that combines visual art with dramatic performance."@en ; skos:definition "Une forme d'art qui combine l'art visuel avec la performance dramatique."@fr ;  skos:closeMatch schema:VisualArtsEvent   ; skos:inScheme adr:ArtsdataEventTypes   .
adr:Conference  rdf:type owl:NamedIndividual , skos:Concept , ado:EventType ; skos:broader  adr:Event ; skos:prefLabel "Conference"@en ; skos:prefLabel "Conférence"@fr ; skos:altLabel "Talk"@en ; skos:definition "A live speaking activity such as a talk and or speech."@en ; skos:definition "Une activité de prise de parole en direct telle qu'une conférence ou un discours."@fr ; skos:note "https://github.com/culturecreates/artsdata-data-model/issues/48" ; skos:inScheme adr:ArtsdataEventTypes   .
adr:Storytelling  rdf:type owl:NamedIndividual , skos:Concept , ado:EventType ; skos:broader  adr:PerformingArtsEvent ; skos:prefLabel "Storytelling"@en ; skos:prefLabel "Conte"@fr ; skos:definition "Storytelling uses words and actions to reveal the elements and images of a story all the while encouraging the listener's imagination."@en ; skos:definition "La Conte utilise des mots et des actions pour révéler les éléments et les images d'une histoire tout en encourageant l'imagination de l'auditeur."@fr ;  skos:exactMatch spt:Conte ;   skos:broadMatch spt:ArtDeLaParole ;  skos:inScheme adr:ArtsdataEventTypes   .
adr:Chanson  rdf:type owl:NamedIndividual , skos:Concept , ado:EventType ; skos:broader  adr:MusicPerformance ; skos:prefLabel "Chanson"@en ; skos:prefLabel "Chanson"@fr ; skos:definition "Performance of lyric-driven songs"@en ; skos:definition "Performance de chanson lyrique"@fr ;  skos:broadMatch spt:Musique ;  skos:inScheme adr:ArtsdataEventTypes   .
adr:Chansonfrancophone  rdf:type owl:NamedIndividual , skos:Concept , ado:EventType ; skos:broader  adr:Chanson ; skos:prefLabel "Chanson francophone"@en ; skos:prefLabel "Chanson francophone"@fr ; skos:definition "Performance of lyric-driven French song"@en ; skos:definition "Performance de chanson française lyrique"@fr ;  skos:broadMatch spt:Musique ;  skos:inScheme adr:ArtsdataEventTypes   .
adr:Chansonanglophone  rdf:type owl:NamedIndividual , skos:Concept , ado:EventType ; skos:broader  adr:Chanson ; skos:prefLabel "English Song"@en ; skos:prefLabel "Chanson anglophone"@fr ; skos:definition "Performance of lyric-driven English song"@en ; skos:definition "Performance de chanson lyrique en anglais"@fr ;  skos:broadMatch spt:Musique ;  skos:inScheme adr:ArtsdataEventTypes   .
adr:JazzShow  rdf:type owl:NamedIndividual , skos:Concept , ado:EventType ; skos:broader  adr:MusicPerformance ; skos:prefLabel "Jazz Show"@en ; skos:prefLabel "Spectacle jazz"@fr ; skos:definition "Jazz music performance"@en ; skos:definition "Un spectacle de musique de jazz"@fr ;  skos:exactMatch spt:Jazz ;  skos:inScheme adr:ArtsdataEventTypes   .
adr:WorldMusicShow  rdf:type owl:NamedIndividual , skos:Concept , ado:EventType ; skos:broader  adr:MusicPerformance ; skos:prefLabel "World Music Show"@en ; skos:prefLabel "Spectacle musique du monde"@fr ; skos:definition "World Music performance"@en ; skos:definition "Spectacle de musique du monde"@fr ;  skos:closeMatch spt:TraditionsDuMonde ;   skos:broadMatch spt:Musique ;  skos:inScheme adr:ArtsdataEventTypes   .
adr:RhythmAndBluesShow  rdf:type owl:NamedIndividual , skos:Concept , ado:EventType ; skos:broader  adr:MusicPerformance ; skos:prefLabel "R&B Show"@en ; skos:prefLabel "Spectacle R&B"@fr ; skos:definition "R&B music performance"@en ; skos:definition "Spectacle de musique R&B"@fr ;  skos:exactMatch spt:RB ;   skos:broadMatch spt:Musique ;  skos:inScheme adr:ArtsdataEventTypes   .
adr:CountryMusicShow  rdf:type owl:NamedIndividual , skos:Concept , ado:EventType ; skos:broader  adr:MusicPerformance ; skos:prefLabel "Country Music Show"@en ; skos:prefLabel "Spectacle de musique country"@fr ; skos:definition "Country music performance"@en ; skos:definition "Performance de musique country"@fr ;  skos:exactMatch spt:Country ;   skos:broadMatch spt:Musique ;  skos:inScheme adr:ArtsdataEventTypes   .
adr:MusicalComedyShow  rdf:type owl:NamedIndividual , skos:Concept , ado:EventType ; skos:broader  adr:MusicalTheatrePerformance ; skos:prefLabel "Musical Comedy Show"@en ; skos:prefLabel "Spectacle comédie musicale"@fr ; skos:definition "A comedic musical theatre peformance"@en ; skos:definition "Un spectacle de théâtre musical comique"@fr ;  skos:closeMatch spt:Musical ;   skos:broadMatch spt:Theatre ;  skos:inScheme adr:ArtsdataEventTypes   .
adr:ClassicalMusicPerformance  rdf:type owl:NamedIndividual , skos:Concept , ado:EventType ; skos:broader  adr:MusicPerformance ; skos:prefLabel "Classical Music Performance"@en ; skos:prefLabel "Spectacle de musique classique"@fr ; skos:definition "A performance of classical music"@en ; skos:definition "Un concert de musique classique"@fr ;  skos:exactMatch spt:Classique ;   skos:broadMatch spt:Musique ;  skos:inScheme adr:ArtsdataEventTypes   .
adr:RockMusicShow  rdf:type owl:NamedIndividual , skos:Concept , ado:EventType ; skos:broader  adr:MusicPerformance ; skos:prefLabel "Rock Music Show"@en ; skos:prefLabel "Spectacle de musique rock"@fr ; skos:definition "A rock music show"@en ; skos:definition "Un spectacle de musique rock"@fr ;  skos:exactMatch spt:Rock ;   skos:broadMatch spt:Musique ;  skos:inScheme adr:ArtsdataEventTypes   .
adr:AcappellaMusicPerformance  rdf:type owl:NamedIndividual , skos:Concept , ado:EventType ; skos:broader  adr:MusicPerformance ; skos:prefLabel "A Cappella Music Show"@en ; skos:prefLabel "Spectacle de musique a capella"@fr ; skos:definition "A performance of a cappella music "@en ; skos:definition "Un spectacle de musique a cappella "@fr ;  skos:broadMatch spt:Musical ;  skos:inScheme adr:ArtsdataEventTypes   .
adr:VarietyShow  rdf:type owl:NamedIndividual , skos:Concept , ado:EventType ; skos:broader  adr:PerformingArtsEvent ; skos:prefLabel "Variety Show"@en ; skos:prefLabel "Spectacle variété"@fr ; skos:definition "Variety show is made up of a variety of acts."@en ; skos:definition "Le spectacle de variétés est composé d'une variété de numéros."@fr ;  skos:exactMatch spt:Variete ;  skos:inScheme adr:ArtsdataEventTypes   .
adr:Classes  rdf:type owl:NamedIndividual , skos:Concept , ado:EventType ; skos:broader  adr:Event ; skos:prefLabel "Classes"@en ; skos:prefLabel "Cours"@fr ; skos:definition "A specialized type of event that is designed for the purpose of providing structured learning experiences offered at specific times and locations."@en ; skos:definition "Un type d'événement spécialisé qui est conçu dans le but de fournir des expériences d'apprentissage structurées offertes à des moments et dans des lieux spécifiques."@fr ;  skos:closeMatch schema:CourseInstance   ; skos:inScheme adr:ArtsdataEventTypes   .
