@prefix owl: <http://www.w3.org/2002/07/owl#> .
@prefix rdf: <http://www.w3.org/1999/02/22-rdf-syntax-ns#> .
@prefix xml: <http://www.w3.org/XML/1998/namespace> .
@prefix xsd: <http://www.w3.org/2001/XMLSchema#> .
@prefix rdfs: <http://www.w3.org/2000/01/rdf-schema#> .
@prefix skos: <http://www.w3.org/2004/02/skos/core#> .
@prefix vann: <http://purl.org/vocab/vann/> .
@prefix schema:  <http://schema.org/> .
@prefix adr:  <http://kg.artsdata.ca/resource/> .

adr:ArtsdataEventCategories rdf:type owl:NamedIndividual, skos:ConceptScheme ;
  skos:prefLabel "Controlled Vocabulary for event types" ;
  rdfs:comment "This SKOS Concept Scheme is a controlled vocabulary for event types (types, categories, disciplines) in Artsdata. The goal of this controlled vocabulary is to serve as a base for mapping different arts organization's event types so events can be reused in event calendars." ;
  owl:versionInfo "3.0.0";
  vann:preferredNamespacePrefix "adr" ;
  vann:preferredNamespaceUri adr: ;
  schema:dateCreated "2021-08-10"^^xsd:date ;
  schema:dateModified "2022-08-01"^^xsd:date ;
  schema:creator  adr:K1-5 ;
  vann:usageNote <https://culturecreates.github.io/artsdata-data-model/classes/event.html> ;
  vann:example ado:PerformingArtsEvent ;
  vann:changes <https://github.com/culturecreates/artsdata-data-model/commits/master/ontology/skos-event-categories.ttl> ; 
  skos:hasTopConcept ado:Event . 

adr:ChildrensEvent  rdf:type owl:NamedIndividual ,  skos:Concept ; skos:broader adr:Event; skos:prefLabel "Children's Event"@en ; skos:prefLabel "Événement pour enfants"@fr ; skos:definition "Event type for children."@en ; skos:definition "Type d'événement : Événement pour enfants"@fr ;schema:about [ a schema:ItemList ; schema:name "Matching Schema.org event type" ; schema:itemListElement  schema:ChildrensEvent  ] ; skos:inScheme adr:ArtsdataEventCategories   .
adr:Event  rdf:type owl:NamedIndividual ,  skos:Concept ; skos:broader adr:Event; skos:prefLabel "Event"@en ; skos:prefLabel "Événement"@fr ; skos:definition "An event is a happening that occurs at a certain time and location. Examples include and are not limited to a: performance, concert, conference, festival, exhibition and/or social gathering."@en ; skos:definition "Un événement est un événement qui se produit à un certain moment et à un certain endroit. Les exemples incluent, sans s'y limiter : une performance, un concert, une conférence, un festival, une exposition et/ou un événement social."@fr ; skos:Note "https://github.com/culturecreates/artsdata-data-model/issues/16" ;schema:about [ a schema:ItemList ; schema:name "Matching Schema.org event type" ; schema:itemListElement  schema:Event  ] ; skos:inScheme adr:ArtsdataEventCategories   .
adr:EventSeries  rdf:type owl:NamedIndividual ,  skos:Concept ; skos:broader adr:Event; skos:prefLabel "Event Series"@en ; skos:prefLabel "Série d'événements"@fr ; skos:definition "An event series is a series of events such as mutiple performances of a same show, or different events grouped by theme. In Schema, included events relate with the series using a superEvent property."@en ; skos:definition "Une série d'événements est une série d'événements connexes tels que plusieurs représentations d'un même spectacle, ou des événements sur un thème. Dans Schema, les événements inclus sont liés à la série à l'aide d'une propriété superEvent."@fr ;schema:about [ a schema:ItemList ; schema:name "Matching Schema.org event type" ; schema:itemListElement  schema:EventSeries  ] ; skos:inScheme adr:ArtsdataEventCategories   .
adr:ExhibitionEvent  rdf:type owl:NamedIndividual ,  skos:Concept ; skos:broader adr:Event; skos:prefLabel "Exhibition"@en ; skos:prefLabel "Exposition"@fr ; skos:definition "An exhibition is a type of event where a collection of objects put together are curated under a theme for the purpose of being presented to a public."@en ; skos:definition "Une exposition est un type d'événement où une collection d'objets rassemblés est organisée sous un thème dans le but d'être présentée à un public."@fr ;schema:about [ a schema:ItemList ; schema:name "Matching Schema.org event type" ; schema:itemListElement  schema:ExhibitionEvent  ] ; skos:inScheme adr:ArtsdataEventCategories   .
adr:Festival  rdf:type owl:NamedIndividual ,  skos:Concept ; skos:broader adr:Event; skos:prefLabel "Festival"@en ; skos:prefLabel "Festival"@fr ; skos:definition "A festival is an organized set of events."@en ; skos:definition "Un festival est un ensemble organisé d'événements."@fr ;schema:about [ a schema:ItemList ; schema:name "Matching Schema.org event type" ; schema:itemListElement  schema:Festival  ] ; skos:inScheme adr:ArtsdataEventCategories   .
adr:MasterclassEvent  rdf:type owl:NamedIndividual ,  skos:Concept ; skos:broader adr:Event; skos:prefLabel "Masterclass"@en ; skos:prefLabel "Cours de maître"@fr ; skos:definition "A masterclass is a class given by an expert in a specific discipline: such as in music, dance, singing, painting or playwrighting."@en ; skos:definition "Une masterclass est un cours donné par un expert dans une discipline spécifique : comme la musique, la danse, le chant, la peinture ou la dramaturgie."@fr ; skos:inScheme adr:ArtsdataEventCategories   .
adr:PerformingArtsEvent  rdf:type owl:NamedIndividual ,  skos:Concept ; skos:broader adr:Event; skos:prefLabel "Performing Arts Event"@en ; skos:prefLabel "Événement des arts de la scène"@fr ; skos:definition "A performing arts event is performing arts work performed for an audience.  It includes a range of performing arts disciplines and genres such as: theatre, ballet, opera, musical theatre, concerts, circus and dance. "@en ; skos:definition "Un événement des arts de la scène est une œuvre des arts de la scène exécutée pour un public. Il comprend une gamme de disciplines et de genres des arts de la scène tels que : le théâtre, le ballet, l'opéra, le théâtre musical, les concerts, le cirque et la danse."@fr ; skos:inScheme adr:ArtsdataEventCategories   .
adr:PublicationEvent  rdf:type owl:NamedIndividual ,  skos:Concept ; skos:broader adr:Event; skos:prefLabel "Publication Event"@en ; skos:prefLabel "Événement de publication"@fr ; skos:definition "Aligning with Schema.org, a PublicationEvent is related to the event of publication of any CreativeWork of any type such as: a broadcast event, an on-demand event, a book/journal publication via a variety of delivery media."@en ; skos:definition "Conformément à Schema.org, un événement de publication est lié à l'événement de publication de tout travail créatif de tout type, tel que : un événement de diffusion, un événement à la demande, une publication de livre/journal via une variété de méthodes médiatiques."@fr ;schema:about [ a schema:ItemList ; schema:name "Matching Schema.org event type" ; schema:itemListElement  schema:PublicationEvent  ] ; skos:inScheme adr:ArtsdataEventCategories   .
adr:RehearsalEvent  rdf:type owl:NamedIndividual ,  skos:Concept ; skos:broader adr:Event; skos:prefLabel "Rehearsal"@en ; skos:prefLabel "Répétition"@fr ; skos:definition "A rehearsal event is an event where the preparation of a performance  is presented to a public."@en ; skos:definition "Un événement de répétition est un événement où la préparation d'un spectacle est présentée à un public."@fr ; skos:inScheme adr:ArtsdataEventCategories   .
adr:ResidencyActivity  rdf:type owl:NamedIndividual ,  skos:Concept ; skos:broader adr:Event; skos:prefLabel "Residency"@en ; skos:prefLabel "Résidence"@fr ; skos:definition "A residency activity is an activity where a sponsor, usually a performing arts organization with access  theatre or venue facility, supports the work of artists by providing resources."@en ; skos:definition "Une activité de résidence est une activité où un sponsor, généralement un organisme des arts de la scène avec accès à un théâtre ou à une salle, soutient le travail des artistes en fournissant des ressources."@fr ; skos:inScheme adr:ArtsdataEventCategories   .
adr:ScreeningEvent  rdf:type owl:NamedIndividual ,  skos:Concept ; skos:broader adr:Event; skos:prefLabel "Screening"@en ; skos:prefLabel "Projection"@fr ; skos:definition "The presentation or showing of a film or video."@en ; skos:definition "La présentation ou la projection d'un film ou d'une vidéo."@fr ;schema:about [ a schema:ItemList ; schema:name "Matching Schema.org event type" ; schema:itemListElement  schema:ScreeningEvent  ] ; skos:inScheme adr:ArtsdataEventCategories   .
adr:SocialEvent  rdf:type owl:NamedIndividual ,  skos:Concept ; skos:broader adr:Event; skos:prefLabel "Social Event"@en ; skos:prefLabel "Événement social"@fr ; skos:definition "A social event is an event organized and planned for a larger group of people."@en ; skos:definition "Un événement social est un événement organisé et planifié pour un plus grand groupe de personnes."@fr ;schema:about [ a schema:ItemList ; schema:name "Matching Schema.org event type" ; schema:itemListElement  schema:SocialEvent  ] ; skos:inScheme adr:ArtsdataEventCategories   .
adr:VisualArtsEvent  rdf:type owl:NamedIndividual ,  skos:Concept ; skos:broader adr:Event; skos:prefLabel "Visual Arts Event"@en ; skos:prefLabel "Événement d'arts visuels"@fr ; skos:definition "Is any event that is related to the discpline of visual arts that includes and is not limited to: ceramics, drawing, painting, photography, digital arts, scuplture, textile arts, conceptual art, film-making, architecture and performance arts."@en ; skos:definition "Est tout événement lié à la discipline des arts visuels qui comprend et ne se limite pas à : la céramique, le dessin, la peinture, la photographie, les arts numériques, la sculpture, les arts textiles, l'art conceptuel, la réalisation de films, l'architecture et les arts de la scène."@fr ;schema:about [ a schema:ItemList ; schema:name "Matching Schema.org event type" ; schema:itemListElement  schema:VisualArtsEvent  ] ; skos:inScheme adr:ArtsdataEventCategories   .
adr:WorkshopEvent  rdf:type owl:NamedIndividual ,  skos:Concept ; skos:broader adr:Event; skos:prefLabel "Workshop"@en ; skos:prefLabel "Atelier"@fr ; skos:definition "A meeting of people to discuss or practice a specific subject or activity."@en ; skos:definition "Une réunion de personnes afin de discuter ou pratiquer un sujet ou une activité spécifique."@fr ; skos:inScheme adr:ArtsdataEventCategories   .
adr:CircusPerformance  rdf:type owl:NamedIndividual ,  skos:Concept ; skos:broader adr:PerformingArtsEvent; skos:prefLabel "Circus"@en ; skos:prefLabel "Cirque"@fr ; skos:definition "A circus is a form of entertainment and spectacle that involves a series of short acts to display human skill, daring, humour and sometimes skilled tricks involving animals.  Often performed in the round under a large tent."@en ; skos:definition "Un cirque est une forme de divertissement et de spectacle qui implique une série de courts numéros pour montrer l'habileté humaine, l'audace, l'humour et parfois des tours impliquant des animaux. Souvent exécuté en rond sous une grande tente."@fr ; skos:Note "https://github.com/culturecreates/artsdata-data-model/issues/7" ; skos:inScheme adr:ArtsdataEventCategories   .
adr:ComedyPerformance  rdf:type owl:NamedIndividual ,  skos:Concept ; skos:broader adr:PerformingArtsEvent; skos:prefLabel "Comedy"@en ; skos:prefLabel "Humour "@fr ; skos:definition "A comedy performance is a form of live entertainment intended to make an audience laugh."@en ; skos:definition "Une comédie est une forme de divertissement destinée à faire rire le public."@fr ;schema:about [ a schema:ItemList ; schema:name "Matching Schema.org event type" ; schema:itemListElement  schema:ComedyEvent  ] ; skos:inScheme adr:ArtsdataEventCategories   .
adr:DancePerformance  rdf:type owl:NamedIndividual ,  skos:Concept ; skos:broader adr:PerformingArtsEvent; skos:prefLabel "Dance"@en ; skos:prefLabel "Danse"@fr ; skos:definition "A dance performance is dance performed for an audience."@en ; skos:definition "Un spectacle de danse est une danse exécutée pour un public."@fr ; skos:Note "https://github.com/culturecreates/artsdata-data-model/issues/23" ;schema:about [ a schema:ItemList ; schema:name "Matching Schema.org event type" ; schema:itemListElement  schema:DanceEvent  ] ; skos:inScheme adr:ArtsdataEventCategories   .
adr:MusicalTheatrePerformance  rdf:type owl:NamedIndividual ,  skos:Concept ; skos:broader adr:PerformingArtsEvent; skos:prefLabel "Musical Theatre"@en ; skos:prefLabel "Théâtre musical"@fr ; skos:definition "Musical theatre is a form of theatrical performance that combines music, singing, dialogue, acting and dance to tell a story. "@en ; skos:definition "Le théâtre musical est une forme de représentation théâtrale qui combine musique, chant, dialogue, jeu d'acteur et danse pour raconter une histoire."@fr ;schema:about [ a schema:ItemList ; schema:name "Matching Schema.org event type" ; schema:itemListElement  schema:TheaterEvent  ] ; skos:inScheme adr:ArtsdataEventCategories   .
adr:MusicPerformance  rdf:type owl:NamedIndividual ,  skos:Concept ; skos:broader adr:PerformingArtsEvent; skos:prefLabel "Music"@en ; skos:prefLabel "Musique"@fr ; skos:definition "A music performance or concert is music performed for an audience."@en ; skos:definition "Une performance musique ou un concert est musique jouée pour un public."@fr ;schema:about [ a schema:ItemList ; schema:name "Matching Schema.org event type" ; schema:itemListElement  schema:MusicEvent  ] ; skos:inScheme adr:ArtsdataEventCategories   .
adr:OperaPerformance  rdf:type owl:NamedIndividual ,  skos:Concept ; skos:broader adr:PerformingArtsEvent; skos:prefLabel "Opera"@en ; skos:prefLabel "Opéra"@fr ; skos:definition "Opera is a form of theatrical performance where music is the fundamental component. Dramatic roles are taken by singers who sing throughout the performance to convey the story."@en ; skos:definition "L'opéra est une forme de représentation théâtrale où la musique est la composante fondamentale. Les rôles dramatiques sont joués par des chanteurs qui chantent tout au long de la représentation pour transmettre l'histoire."@fr ;schema:about [ a schema:ItemList ; schema:name "Matching Schema.org event type" ; schema:itemListElement  schema:MusicEvent  ] ; skos:inScheme adr:ArtsdataEventCategories   .
adr:SpokenWordPerformance  rdf:type owl:NamedIndividual ,  skos:Concept ; skos:broader adr:PerformingArtsEvent; skos:prefLabel "Spoken Word"@en ; skos:prefLabel "Mot parlé"@fr ; skos:definition "A spoken word is a designation for poetry that is performed for a public."@en ; skos:definition "Un mot parlé est une désignation pour la poésie qui est exécutée pour un public."@fr ;schema:about [ a schema:ItemList ; schema:name "Matching Schema.org event type" ; schema:itemListElement  schema:TheaterEvent  ] ; skos:inScheme adr:ArtsdataEventCategories   .
adr:TheatrePerformance  rdf:type owl:NamedIndividual ,  skos:Concept ; skos:broader adr:PerformingArtsEvent; skos:prefLabel "Theatre"@en ; skos:prefLabel "Théâtre"@fr ; skos:definition "A theatre performance is theatre work performed for an audience."@en ; skos:definition "Une représentation théâtrale est une pièce de théâtre jouée pour un public."@fr ;schema:about [ a schema:ItemList ; schema:name "Matching Schema.org event type" ; schema:itemListElement  schema:TheaterEvent  ] ; skos:inScheme adr:ArtsdataEventCategories   .
adr:BroadcastEvent  rdf:type owl:NamedIndividual ,  skos:Concept ; skos:broader adr:PublicationEvent; skos:prefLabel "Broadcast"@en ; skos:prefLabel "Diffusion"@fr ; skos:definition "It is a one-to-many distribution of video and/or audio content via a electronic mass communication method. The content may be livestreamed or pre-recorded."@en ; skos:definition "Il s'agit d'une distribution un-à-plusieurs de contenu vidéo et/ou audio via une méthode de communication électronique de masse. Le contenu peut être diffusé en direct ou pré-enregistré."@fr ; skos:Note "https://github.com/culturecreates/artsdata-data-model/issues/30" ;schema:about [ a schema:ItemList ; schema:name "Matching Schema.org event type" ; schema:itemListElement  schema:BroadcastEvent  ] ; skos:inScheme adr:ArtsdataEventCategories   .
adr:LiveBroadcastEvent  rdf:type owl:NamedIndividual ,  skos:Concept ; skos:broader adr:BroadcastEvent; skos:prefLabel "Live Stream"@en ; skos:prefLabel "Diffusion en direct"@fr ; skos:definition "A livestream broadcast of video and/or audio content via a electronic mass communication method. "@en ; skos:definition "Une diffusion en direct de contenu vidéo et/ou audio via un procédé de communication électronique de masse."@fr ; skos:inScheme adr:ArtsdataEventCategories   .
adr:OnDemand  rdf:type owl:NamedIndividual ,  skos:Concept ; skos:broader adr:PublicationEvent; skos:prefLabel "On Demand"@en ; skos:prefLabel "Sur demande"@fr ; skos:definition "As per Schema.org, this is a publication event during which a program (e.g. catch-up TV or radio podcast) is available on-demand."@en ; skos:definition "Selon Schema.org, il s'agit d'un événement de publication au cours duquel un programme (par exemple, une télévision de rattrapage ou un podcast radio) est disponible à la demande."@fr ;schema:about [ a schema:ItemList ; schema:name "Matching Schema.org event type" ; schema:itemListElement  schema:OnDemandEvent  ] ; skos:inScheme adr:ArtsdataEventCategories   .
adr:PostshowTalk  rdf:type owl:NamedIndividual ,  skos:Concept ; skos:broader adr:Event; skos:prefLabel "Postshow Talk"@en ; skos:prefLabel "Conférence après-spectacle"@fr ; skos:definition "An informative talk with an audience after a performance"@en ; skos:definition "Une discussion informative avec un public après une représentation"@fr ;schema:about [ a schema:ItemList ; schema:name "Matching Schema.org event type" ; schema:itemListElement  schema:Event  ] ; skos:inScheme adr:ArtsdataEventCategories   .
adr:PreshowTalk  rdf:type owl:NamedIndividual ,  skos:Concept ; skos:broader adr:Event; skos:prefLabel "Preshow Talk"@en ; skos:prefLabel "Conférence avant-spectacle"@fr ; skos:definition "An informative talk with an audience before a performance"@en ; skos:definition "Une discussion informative avec un public avant une représentation"@fr ;schema:about [ a schema:ItemList ; schema:name "Matching Schema.org event type" ; schema:itemListElement  schema:Event  ] ; skos:inScheme adr:ArtsdataEventCategories   .
adr:PerformanceArt  rdf:type owl:NamedIndividual ,  skos:Concept ; skos:broader adr:VisualArtsEvent; skos:prefLabel "Performance Art"@en ; skos:prefLabel "Art performance"@fr ; skos:definition "An art form that combines visual art with dramatic performance."@en ; skos:definition "Une forme d'art qui combine l'art visuel avec la performance dramatique."@fr ;schema:about [ a schema:ItemList ; schema:name "Matching Schema.org event type" ; schema:itemListElement  schema:VisualArtsEvent  ] ; skos:inScheme adr:ArtsdataEventCategories   .